Update turing_machine.lean

scripts/turing_machine.lean
@@ -6,20 +6,19 @@ structure TuringMachine where /- generalizes to tapes besides ℤ obviously 💅
   translate: tape × shift → tape
   update: state × symbol → state × symbol × shift
 
-structure DynamicalSystem where
+structure DiscreteDynamicalSystem where
   state: Type
   update: state → state
 
-def TuringMachineToDynamicalSystem (M: TuringMachine) [DecidableEq M.tape]: DynamicalSystem := {
+example (M: TuringMachine) [DecidableEq M.tape]: DiscreteDynamicalSystem := {
   state := (M.tape → M.symbol) × M.state × M.tape
-  update := fun (u, s, x) => by {
+  update := fun (u, s, x) => by
     have (y1, y2, y3) := M.update (s, (u x))
     exact (
       fun x0 => if x = x0 then y2 else (u x0),
       y1,
       M.translate (x, y3)
     )
-  }
 }
 
 /- some theorem to cap it off? -/
